updated cstack

CStack.v
@@ -2,6 +2,7 @@ Require Import CUtils.
 Require Import List.
 Require Import String.
 Require Import Arith.
+Require Import Omega.
 Require Import PartialMaps.
 Import ListNotations.
 
@@ -27,25 +28,51 @@ Fixpoint replace_addr_s (s: cstack) (addr newval: nat):
                f::(replace_addr_s s' (addr - List.length f) newval)
   end.
 
-Definition lookup_addr_s (s: cstack) (addr: nat): option nat.
-Admitted.
+Fixpoint lookup_addr_s (s: cstack) (addr: nat): option nat :=
+  match s with
+  | [] => None
+  | f::s' => if (addr <? List.length f) then
+               lookup_addr f addr
+             else
+               lookup_addr_s s' (addr - List.length f)
+  end.
 
-Definition get_addr_s (st: stack sym_tbl) (var: string): option nat.
-Admitted.
+Fixpoint get_addr_s (st: stack sym_tbl) (var: string): option nat :=
+  match st with
+  | [] => None
+  | ft::st' => match ft var with
+               | None => get_addr_s st' var
+               | Some val => Some val
+               end
+  end.
 
-Definition lookup_var_s (s: cstack) (st: stack sym_tbl) (var: string) : option nat.
-Admitted.
+Definition lookup_var_s (s: cstack) (st: stack sym_tbl) (var: string) : option nat :=
+  match get_addr_s st var with
+  | None => None
+  | Some addr => lookup_addr_s s addr
+  end.
 
-Definition valid_state_s (s: cstack) (st: stack sym_tbl): Prop.
-Admitted.
+(* Important properties of validity for stacks:
+   * The stack and stack symbol table are the same length.
+   * each frame is valid 
+**)
+Fixpoint valid_state_s (s: cstack) (st: stack sym_tbl): Prop :=
+  match s, st with
+  | f::s', ft::st' => valid_state_f f ft /\ (valid_state_s s' st')
+  | [], [] => True
+  | _, _ => False
+  end.
 
 Definition push_frame_s (s: cstack) (st: stack sym_tbl):
-  (cstack*stack sym_tbl).
-Admitted.
+  (cstack*stack sym_tbl) :=
+  ([]::s, empty::st).  
 
 Definition pop_frame_s (s: cstack) (st: stack sym_tbl):
-  (cstack * stack sym_tbl).
-Admitted.
+  (cstack * stack sym_tbl) :=
+  match s, st with
+  | _::s', _::st' => (s', st')
+  | _, _ => ([], [])
+  end.
 
 Inductive cstack_frame_seq:
   cstack -> stack sym_tbl -> cstack -> stack sym_tbl -> Prop :=
@@ -63,9 +90,41 @@ Inductive cstack_frame_seq:
     cstack_frame_seq s' st' s'' st'' ->
     cstack_frame_seq s st s'' st''.
 
+Inductive cstack_frame_seq_limit_pop:
+  cstack -> stack sym_tbl -> cstack -> stack sym_tbl -> string -> Prop :=
+| cstack_frame_limit_pop_refl: forall s st limited,
+    valid_state_s s st ->
+    cstack_frame_seq_limit_pop s st s st limited
+| cstack_frame_limit_pop_newframe: forall s st limited,
+    valid_state_s s st ->
+    cstack_frame_seq_limit_pop s st ([]::s) (empty::st) limited
+| cstack_frame_limit_pop_popframe: forall s st f ft limited,
+    valid_state_s (f::s) (ft::st) ->
+    ft limited = None ->
+    cstack_frame_seq_limit_pop (f::s) (ft::st) s st limited
+| cstack_frame_limit_pop_trans: forall s st s' st' s'' st'' limited,
+    cstack_frame_seq_limit_pop s st s' st' limited ->
+    cstack_frame_seq_limit_pop s' st' s'' st'' limited ->
+    cstack_frame_seq_limit_pop s st s'' st'' limited.  
+  
+
+(* Essentially, there are two sets of each operation 
+   provided. 
+
+   There is a sequence definition which is written in terms of 
+   the operations that a cstack has.
+
+   The second sequence definition is reworded so that it it relies
+   on the commutativity property of insertions / frame operations 
+   to cluster by frame.  (These are wrapper)
+
+   The reason why we do this is because the second version is much easier to prove with, but the first version is what we want to use.
+**)
+
 Inductive cstack_seq:
   cstack -> stack sym_tbl -> cstack -> stack sym_tbl -> Prop :=
 | cstack_refl: forall s st,
+    valid_state_s s st ->
     cstack_seq s st s st
 | cstack_var: forall f s ft st f' ft',
     valid_state_s (f::s) (ft::st) ->
@@ -83,6 +142,7 @@ Inductive cstack_no_rewrite:
   cstack -> stack sym_tbl -> cstack -> stack sym_tbl -> nat ->
   Prop :=
 | cstack_no_rewrite_refl: forall s st n,
+    valid_state_s s st ->
     cstack_no_rewrite s st s st n
 | cstack_no_rewrite_addr: forall f s ft st f' ft' addr,
     valid_state_s s st ->
@@ -101,6 +161,7 @@ Inductive cstack_no_shadowing:
   cstack -> stack sym_tbl -> cstack -> stack sym_tbl -> string ->
   Prop :=
 | cstack_no_shadowing_refl: forall s st var,
+    valid_state_s s st ->
     cstack_no_shadowing s st s st var
 | cstack_no_shadowing_addr: forall f s ft st f' ft' var,
     valid_state_s (f::s) (ft::st) ->
@@ -108,7 +169,7 @@ Inductive cstack_no_shadowing:
     frame_seq_lift_insert_var f ft f' ft' var ->
     cstack_no_shadowing (f::s) (ft::st) (f'::s) (ft'::st) var
 | cstack_no_shadowing_frame: forall s st s' st' var,
-    cstack_frame_seq s st s' st' ->
+    cstack_frame_seq_limit_pop s st s' st' var ->
     cstack_no_shadowing s st s' st' var
 | cstack_no_shadowing_trans: forall s st s' st' s'' st'' var,
     cstack_no_shadowing s st s' st' var ->
@@ -196,6 +257,24 @@ Inductive cstack_seq_wrapper_no_rewrite:
     cstack_seq_wrapper_no_rewrite s' st' s'' st'' oldaddr ->
     cstack_seq_wrapper_no_rewrite s st s'' st'' oldaddr.
 
+Lemma valid_state_s_len: forall s st,
+    valid_state_s s st ->
+    List.length s = List.length st.
+Proof.
+  induction s; intros.
+  - unfold valid_state_s in H.
+    destruct st; [reflexivity | contradiction].
+  - simpl in *.
+    destruct st.
+    + contradiction.
+    + simpl. f_equal. apply IHs. destruct H as [_ H]. assumption.
+Qed.
+
+Theorem limit_pop_imp_frame_seq: forall s st s' st' limited,
+    cstack_frame_seq_limit_pop s st s' st' limited ->
+    cstack_frame_seq s st s' st'.
+Admitted.
+
 Theorem cstack_wrapper_imp_cstack: forall s st s' st',
     cstack_seq_wrapper s st s' st' <->
     cstack_seq s st s' st'.
@@ -218,33 +297,187 @@ Theorem cstack_no_rewrite_imp_cstack: forall s st s' st' addr,
     cstack_no_rewrite s st s' st' addr ->
     cstack_seq s st s' st'.
 Proof.
-Admitted.
+  intros.
+  induction H; intros.
+  - apply cstack_refl. assumption.
+  - apply cstack_var.
+    
 
 Theorem cstack_no_shadowing_imp_cstack: forall s st s' st' var,
     cstack_no_shadowing s st s' st' var ->
     cstack_seq s st s' st'.
 Proof.
-Admitted.
+  intros.
+  induction H; intros.
+  - apply cstack_refl. assumption.
+  - apply cstack_var.
+    assumption.
+    apply lift_insert_imp_frame_seq with (targetvar:=var).
+    assumption.
+  - apply cstack_frame.
+    apply limit_pop_imp_frame_seq with (limited:=var).
+    assumption.
+  - eapply cstack_trans.
+    apply IHcstack_no_shadowing1.
+    apply IHcstack_no_shadowing2.
+Qed.
+
+(* These are the theorems that provide information **)
+
+Theorem preservation_cstack_frame_seq: forall
+    s st s' st',
+    cstack_frame_seq s st s' st' ->
+    valid_state_s s' st'.
+Proof.
+  intros.
+  induction H; intros.
+  - assumption.
+  - simpl. split. apply valid_state_f_empty.
+    assumption.
+  - inversion H. assumption.
+  - assumption.
+Qed.
+
+Theorem cstack_frame_seq_lookup_correct: forall
+    s st s' st' var addr,
+    get_addr_s st var = Some addr ->
+    cstack_frame_seq_limit_pop s st s' st' var ->
+    get_addr_s st' var = Some addr.
+Proof.
+  intros.
+  induction H0; intros.
+  - assumption.
+  - assumption.
+  - simpl in H. rewrite H1 in H.
+    assumption.
+  - apply IHcstack_frame_seq_limit_pop2.
+    apply IHcstack_frame_seq_limit_pop1.
+    assumption.
+Qed.
 
 Theorem preservation_valid_state_s: forall
     s st s' st',
     cstack_seq s st s' st' ->
     valid_state_s s' st'.
 Proof.
-Admitted.
+  intros.
+  induction H; intros.
+  - assumption.
+  - inversion H.
+    simpl. split.
+    apply (preservation_valid_state_f f ft).
+    assumption.
+    assumption.
+  - apply (preservation_cstack_frame_seq s st).
+    assumption.
+  - assumption.
+Qed.  
 
 Theorem cstack_seq_lookup_correct: forall
     s st s' st' var addr,
     get_addr_s st var = Some addr ->
     cstack_no_shadowing s st s' st' var ->
-    get_addr_s st var = Some addr.
+    get_addr_s st' var = Some addr.
 Proof.
-Admitted.
+  intros.
+  induction H0; intros.
+  - assumption.
+  - simpl in *.
+    erewrite frame_seq_lookup_correct. reflexivity.
+
+    destruct (ft var) eqn:eq.
+    rewrite H in eq. apply eq.
+    congruence.
+
+    apply lift_insert_imp_frame_seq in H2.
+    apply H2.
+  - apply (cstack_frame_seq_lookup_correct s st s'); assumption.
+  - apply IHcstack_no_shadowing2.
+    apply IHcstack_no_shadowing1.
+    assumption.
+Qed.
+
+Fixpoint stack_size (s: cstack): nat :=
+  match s with
+  | [] => 0
+  | h::t => (List.length h) + (stack_size t)
+  end.
+
+Lemma append_frame_size: forall (s: cstack) (f f': frame),
+    stack_size (f'::s) - stack_size(f::s) =
+    List.length f' - List.length f.
+Proof.
+  intros. simpl. omega.
+Qed.
+
+Lemma append_frame_comp: forall (s: cstack) (f f': frame),
+    stack_size (f'::s) >= stack_size (f::s) ->
+    List.length f' >= List.length f.
+Proof.
+  intros.
+  simpl in *. omega.
+Qed.
 
 Theorem cstack_seq_no_rewrite_correct: forall
     s st s' st' addr val,
-    lookup_addr_s s addr = val ->
+    lookup_addr_s s addr = Some val ->
     cstack_no_rewrite s st s' st' addr ->
-    lookup_addr_s s addr = val.
+    stack_size s' >= stack_size s ->
+    lookup_addr_s s' (stack_size s' - stack_size s + addr) = Some val.
 Proof.
+  intros.
+  assert (valid_state_s s' st'). {
+    apply preservation_valid_state_s with (s:=s) (st:=st).
+    apply cstack_no_rewrite_imp_cstack with (addr:=addr).
+    assumption.
+  }
+  induction H0; subst.
+  - rewrite Nat.sub_diag. simpl. assumption.
+  - rewrite append_frame_size.
+    apply append_frame_comp in H1.
+    simpl in *.
+
+    destruct (addr <? Datatypes.length f) eqn:eq.
+
+    rewrite Nat.ltb_lt in eq.
+    apply (plus_lt_compat_l _ _ (Datatypes.length f' - Datatypes.length f)) in eq.
+    assert (Datatypes.length f' - Datatypes.length f +
+            Datatypes.length f = Datatypes.length f'). omega.
+    rewrite H4 in eq. clear H4.
+    rewrite <- Nat.ltb_lt in eq.
+    rewrite eq.
+    eapply frame_seq_no_rewrite_correct.
+    destruct H2 as [fH sH].
+    unfold valid_state_f in fH.
+    assumption.
+    apply H3.
+
+    rewrite Nat.ltb_ge in eq.
+    apply (plus_le_compat_l _ _ (Datatypes.length f' - Datatypes.length f)) in eq.
+    assert (Datatypes.length f' - Datatypes.length f +
+            Datatypes.length f = Datatypes.length f'). omega.
+    rewrite H4 in eq.
+    rewrite <- Nat.ltb_ge in eq.
+    rewrite eq.
+
+    assert (Datatypes.length f' - Datatypes.length f + addr -
+                                                       Datatypes.length f' = addr - Datatypes.length f).
+    omega.
+    rewrite H5.
+    assumption.
+  - induction H0.
+    + rewrite Nat.sub_diag. simpl. assumption.
+    + simpl. rewrite Nat.sub_diag. simpl. rewrite Nat.sub_0_r. assumption.
+    + simpl in *.
+      assert (f = []). {
+        apply length_zero_iff_nil.
+        omega.
+      }
+
+      rewrite H3.
+      simpl. rewrite Nat.sub_diag. simpl.
+      rewrite H3 in H. simpl in H. rewrite Nat.sub_0_r in H. assumption.
+    + admit.
+  - admit.
 Admitted.
+    
