CUtils.v
@@ -1,35 +1,47 @@
 Require Import PartialMaps.
 Require Import String.
+Require Import List.
+Require Import Omega.
+Import ListNotations.
 
 Definition sym_tbl := partial_map string nat.
 
-(* Can imagine a heap as a single stack frame **)
 Definition stack (A: Type) := list A.
 
 Definition frame := stack nat.
 
+(* Use this to create a new variable in a frame **)
 Definition insert_var (f: frame)
            (ft: sym_tbl) (var: string) (val: nat)
-  : (frame * sym_tbl).
-Admitted.
+  : (frame * sym_tbl) :=
+  (val::f, (var |-> List.length f; ft)).
 
-Definition replace_addr (f: frame) (addr newval: nat)
-  : frame.
-Admitted.
+Fixpoint replace_addr (f: frame) (addr newval: nat)
+  : frame :=
+  match f with
+  | [] => []
+  | h::t => match addr with
+            | 0 => newval::t
+            | S n => h::(replace_addr t n newval)
+            end
+  end.
 
-Definition lookup_addr (f: frame) (addr: nat) : option nat.
-Admitted.
+Definition lookup_addr (f: frame) (addr: nat) : option nat :=
+  nth_error f addr.
 
+Hint Unfold lookup_addr.
 
 Definition lookup_var (f: frame) (ft: sym_tbl) (var: string) : option nat :=
   match ft var with
   | None => None
-  | Some addr => lookup_addr f addr
+  | Some addr => lookup_addr f (List.length f - addr)
   end.
 
 
 Definition valid_state_f (f: frame) (ht: sym_tbl): Prop :=
-  True.
+  forall var addr, ht var = Some addr -> addr < List.length f.
+
+Hint Unfold valid_state_f.
 
 (* for a regular heap, use offset of 0.  used to create frames **)
 Inductive frame_seq:
@@ -76,60 +88,183 @@ Inductive frame_seq_no_rewrite:
 
 Inductive frame_seq_lift_insert_var:
   frame -> sym_tbl -> frame -> sym_tbl -> string -> Prop :=
-| frame_exclude_var_refl: forall (f: frame) (ft: sym_tbl) targetvar,
+| frame_lift_var_refl: forall (f: frame) (ft: sym_tbl) targetvar,
     valid_state_f f ft ->
     frame_seq_lift_insert_var f ft f ft targetvar
-| frame_live_insert_var_insert: forall f ft f' ft' val targetvar,
+| frame_lift_insert_var: forall f ft f' ft' val targetvar,
     valid_state_f f ft ->
     ft targetvar = None ->
     insert_var f ft targetvar val = (f', ft')->
     frame_seq_lift_insert_var f ft f' ft' targetvar
-| frame_lift_insert_var_update_addr:
+| frame_lift_update_addr:
     forall f ft f' addr newval targetvar,
     valid_state_f f ft ->
     0 <= addr < List.length f ->
     replace_addr f addr newval = f' ->
     frame_seq_lift_insert_var f ft f' ft targetvar
-| frame_lift_insert_trans: forall f ft f' ft' f'' ft'' targetvar,
+| frame_lift_trans: forall f ft f' ft' f'' ft'' targetvar,
     frame_seq_lift_insert_var f ft f' ft' targetvar ->
     frame_seq_lift_insert_var f' ft' f'' ft'' targetvar ->
     frame_seq_lift_insert_var f ft f'' ft'' targetvar.
 
-Theorem lif_insert_imp_frame_seq: forall f ft f' ft' targetvar,
-    frame_seq_no_rewrite f ft f' ft' targetvar ->
+Lemma nth_error_nil: forall A addr,
+    @nth_error A [] addr = None.
+Proof.
+  intros.
+  destruct addr; reflexivity.
+Qed.
+
+
+(* Some lemmas about home cooked replacement **)
+Lemma replace_addr_len: forall f addr newval,
+    List.length f = List.length (replace_addr f addr newval).
+Proof.
+  induction f; intros.
+  - reflexivity.
+  - simpl.
+    destruct addr.
+    + reflexivity.
+    + simpl. f_equal. apply IHf.
+Qed.
+
+Lemma replace_addr_lookup_eq: forall f addr newval,
+    0 <= addr < List.length f ->
+    lookup_addr (replace_addr f addr newval) addr = Some newval.
+Proof.
+  induction f; intros.
+  - simpl in H. inversion H. inversion H1.
+  - simpl in *.
+    destruct addr.
+    + reflexivity.
+    + simpl.
+      apply IHf.
+      omega.
+Qed.
+
+Lemma replace_addr_lookup_neq: forall f addr oldaddr newval,
+    addr <> oldaddr ->
+    lookup_addr (replace_addr f addr newval) oldaddr = lookup_addr f oldaddr.
+Proof.
+  induction f; intros.
+  - reflexivity.
+  - simpl.
+    destruct addr.
+    + unfold lookup_addr.
+      destruct oldaddr; try contradiction.
+      reflexivity.
+    + destruct oldaddr.
+      * reflexivity.
+      * simpl. apply IHf. omega.
+Qed.  
+
+Theorem lift_insert_imp_frame_seq: forall f ft f' ft' targetvar,
+    frame_seq_lift_insert_var f ft f' ft' targetvar ->
     frame_seq f ft f' ft'.
 Proof.
-Admitted.
-
+  intros. induction H; subst.
+  - apply frame_refl. assumption.
+  - apply frame_insert with (var:=targetvar) (val:=val); assumption.
+  - apply frame_update_addr with (addr:=addr) (newval:=newval); try assumption; try reflexivity.
+  - eapply frame_trans.
+    apply IHframe_seq_lift_insert_var1.
+    assumption.
+Qed.
 
 Theorem no_rewrite_imp_frame_seq: forall f ft f' ft' n,
     frame_seq_no_rewrite f ft f' ft' n ->
     frame_seq f ft f' ft'.
 Proof.
-Admitted.
+  intros.
+  induction H; subst.
+  - apply frame_refl. assumption.
+  - apply frame_insert with (var:=var) (val:=val); assumption.
+  - apply frame_update_addr with (addr:=addr) (newval:=newval);
+      try assumption; try reflexivity.
+  - eapply frame_trans.
+    apply IHframe_seq_no_rewrite1.
+    assumption.
+Qed.
+
+Theorem valid_state_f_empty: valid_state_f [] ({}).
+Proof.
+  unfold valid_state_f.
+  intros.
+  inversion H.
+Qed.
 
 Theorem preservation_valid_state_f: forall
     f ft f' ft',
     frame_seq f ft f' ft' ->
     valid_state_f f' ft'.
 Proof.
-Admitted.
+  intros. 
+  induction H.
+  - assumption.
+  - inversion H1; subst; clear H1.
+    unfold valid_state_f; intros.
+    destruct (string_dec var var0).
+    + rewrite e in H1. rewrite update_eq in H1.
+      inversion H1; subst; clear H1.
+      simpl. omega.
+    + rewrite update_neq in H1. 2: auto.
+      unfold valid_state_f in H.
+      simpl.
+      specialize H with (var:=var0) (addr:=addr).
+      apply H in H1.
+      omega.
+  - inversion H1; subst; clear H2.
+    unfold valid_state_f; intros.
+    rewrite <- (replace_addr_len _ addr newval).
+    unfold valid_state_f in H.
+    apply (H var _ H1).
+  - assumption.
+Qed.  
 
 Theorem frame_seq_lookup_correct: forall
     f ft f' ft' var addr,
-    ft var = addr ->
+    ft var = Some addr ->
     frame_seq f ft f' ft' ->
-    ft' var = addr.
+    ft' var = Some addr.
 Proof.
-Admitted.
-
+  intros.
+  induction H0; intros.
+  - assumption.
+  - inversion H2; subst; clear H2.
+    destruct (string_dec var0 var).
+    + congruence.
+    + rewrite update_neq. 2: auto.
+      assumption.
+  - assumption.
+  - auto.
+Qed.
 
 Theorem frame_seq_no_rewrite_correct: forall
     f ft f' ft' addr val,
     lookup_addr f addr = val ->
     frame_seq_no_rewrite f ft f' ft' addr ->
-    lookup_addr f addr = val.
+    lookup_addr f' (List.length f' - List.length f + addr) = val.
 Proof.
+  intros.
+  induction H0; intros.
+  - rewrite Nat.sub_diag.
+    simpl. assumption.
+  - inversion H2; subst; clear H2.
+    unfold lookup_addr.
+
+    assert (List.length (val0::f) - Datatypes.length f = 1). {
+      simpl.
+      destruct (List.length f); omega.
+    }
+
+    rewrite H. reflexivity.
+  - rewrite <- H.
+    rewrite <- H3.
+    rewrite <- (replace_addr_len f addr newval).
+
+    rewrite Nat.sub_diag. simpl.
+    apply replace_addr_lookup_neq. assumption.
+  - admit.
 Admitted.
-
-
+    
+    
+    
